Remove syntactic types

linear_semtype.v
@@ -1,26 +1,24 @@
 From pv Require Import proofmode.
 
-Print ty.
-
-Definition TExcept : tag -> val -> sepProp := fun _ v =>
+Definition EPhi (t : tag) (v : val) : sepProp :=
   (Ex n, @[ v = VNat n ]) ** TRUE.
 
-Fixpoint sem (A : ty) (v : val) : sepProp :=
-  match A with
-  | TUnit => @[ v = VUnit ]
-  | TNat => Ex n, @[ v = VNat n ]
-  | TBool => Ex b, @[ v = VBool b ]
-  | TMoved => EMP
-  | TRef A => Ex l w, @[ v = VRef l ] ** l ~> w ** sem A w
-  | TProd A1 A2 => Ex w1 w2, @[ v = VPair w1 w2 ] ** sem A1 w1 ** sem A2 w2
-  | TSum A1 A2 => (Ex w : val, @[v = VInjL w] ** sem A1 w) \//
-                  (Ex w : val, @[v = VInjR w] ** sem A2 w)
-  | TFun A1 A2 => 
-      @[ forall w, sem A1 w |~ 
-          wp (EApp (EVal v) (EVal w)) (fun v => sem A2 v ** TRUE) TExcept ]
-  | TFunOnce A1 A2 => 
-      All w, sem A1 w -** wp (EApp (EVal v) (EVal w)) (fun v => sem A2 v ** TRUE) TExcept
-  end.
+Definition ty := val -> sepProp.
+
+Definition TUnit : ty := fun v => @[ v = VUnit ].
+Definition TNat : ty := fun v => Ex n, @[ v = VNat n ].
+Definition TBool : ty := fun v => Ex b, @[ v = VBool b ].
+Definition TMoved : ty := fun v => EMP.
+Definition TRef (A : ty) : ty := fun v =>
+  Ex l w, @[ v = VRef l ] ** l ~> w ** A w.
+Definition TProd (A1 A2 : ty) : ty := fun v =>
+  Ex w1 w2, @[ v = VPair w1 w2 ] ** A1 w1 ** A2 w2.
+Definition TSum (A1 A2 : ty) : ty := fun v =>
+  Ex w, (@[ v = VInjL w ] ** A1 w) \// (@[ v = VInjR w] ** A2 w).
+Definition TFun (A1 A2 : ty) : ty := fun v =>
+  @[ forall w, A1 w |~ wp (EApp (EVal v) (EVal w)) A2 EPhi ].
+Definition TFunOnce (A1 A2 : ty) : ty := fun v =>
+  All w, A1 w -** wp (EApp (EVal v) (EVal w)) A2 EPhi.
 
 (** Intuitively, contexts are multisets of bindings (since variables can occur
 multiple times). We formalize contexts in Coq as lists. The lemma [subctx_swap]
@@ -41,27 +39,27 @@ to ensure the ownership of all variables in the context is separate. *)
 Fixpoint ctx_typed (Gamma : ty_ctx) (vs : stringmap val) : sepProp :=
   match Gamma with
   | [] => EMP
-  | (x,A) :: Gamma =>
-     (Ex v, @[ StringMap.lookup vs x = Some v ] ** sem A v) **
-     ctx_typed Gamma vs
+  | (x, A) :: Gamma =>
+      (Ex v, @[ StringMap.lookup vs x = Some v ] ** A v) **
+      ctx_typed Gamma vs
   end.
 
 (** The semantic typing judgments are defined similarly to the ones from week 6,
 but using separation logic entailment [|~] instead of a Coq implication. *)
 
 Definition val_typed (v : val) (A : ty) : Prop :=
-  TRUE |~ sem A v ** TRUE.
+  TRUE |~ A v ** TRUE.
 
 Definition typed (Gamma : ty_ctx) (e : expr) (A : ty) : Prop :=
   forall vs,
-    ctx_typed Gamma vs |~ 
-      wp (subst_map vs e) (fun v => sem A v ** TRUE) TExcept.
+    ctx_typed Gamma vs |~
+      wp (subst_map vs e) (fun v => A v ** TRUE) EPhi.
 
 Definition copy (A : ty) : Prop :=
-  forall v, sem A v |~ @[ EMP |~ sem A v ].
+  forall v, A v |~ @[ EMP |~ A v ].
 
 Definition subty (A1 A2 : ty) : Prop :=
-  forall v, sem A1 v |~ sem A2 v.
+  forall v, A1 v |~ A2 v.
 
 (** We lift subtyping to contexts. This allows us to:
 
@@ -104,73 +102,3 @@ Proof.
     destruct Hfresh; auto.
   - iApply ("IH" with "[%] Hctx"). tauto.
 Qed.
-
-Lemma Closure_typed x e A1 A2 :
-  typed [(x,A1)] e A2 ->
-  val_typed (VClosure x e) (TFun A1 A2).
-Proof. 
-  iIntros "%Htyped Htrue". iSplitR;[|done].
-  iIntros "!% %w Hw". iApply App_wp. 
-  rewrite <- subst_map_singleton.
-  iApply Htyped. unfold ctx_typed;iSplitL;[|done].
-  iExists w. iFrame. iPureIntro;StringMap.map_solver.
-Qed. 
-
-Lemma App_typed Gamma1 Gamma2 e1 e2 A B :
-  typed Gamma1 e1 (TFunOnce A B) ->
-  typed Gamma2 e2 A ->
-  typed (Gamma1 ++ Gamma2) (EApp e1 e2) B.
-Proof.
-  iIntros "%He1 %He2 %vs Hctx" .
-  iDestruct (ctx_typed_app with "Hctx") as "[Hctx1 Hctx2]";simpl.
-  iApply (He1 with "Hctx1"). iSplit.
-  { iIntros (v1) "[Hv1 Htrue]". iApply (He2 with "Hctx2"). iSplit.
-    + iIntros (v2) "[Hv2 Htrue2]";simpl.
-
-Qed.
-
-Lemma Lam_typed Gamma e x A1 A2 :
-  ~In x (ctx_dom Gamma) ->
-  typed ((x,A1) :: Gamma) e A2 ->
-  typed Gamma (ELam x e) (TFunOnce A1 A2).
-Proof.
-  unfold typed. iIntros (? He vs) "Hctx". simpl.
-  iApply Lam_wp. iIntros (w) "HA". iApply App_wp.
-  (** We need to turn the [subst] into a [substmap] so that we can [iApply]
-  the hypothesis [He]. *)
-  rewrite <-subst_map_insert.
-
-  iApply He; simpl. iSplitL "HA".
-  { iExists w. iFrame. iPureIntro. StringMap.map_solver. }
-  by iApply ctx_typed_insert.
-Qed.
-
-Lemma If_typed Gamma1 Gamma2 e1 e2 e3 B :
-  typed Gamma1 e1 TBool ->
-  typed Gamma2 e2 B ->
-  typed Gamma2 e3 B ->
-  typed (Gamma1 ++ Gamma2) (EIf e1 e2 e3) B.
-Proof.
-  unfold typed. iIntros (He1 He2 He3 vs) "Hctx". simpl.
-  iDestruct (ctx_typed_app with "Hctx") as "[Hctx1 Hctx2]".
-  iApply (He1 with "Hctx1"). iIntros (v1) "[%b ->]". destruct b.
-  - iApply If_true_wp. by iApply He2.
-  - iApply If_false_wp. by iApply He3.
-Qed.
-
-Lemma Seq_typed Gamma1 Gamma2 e1 e2 A B :
-  copy A ->
-  typed Gamma1 e1 A ->
-  typed Gamma2 e2 B ->
-  typed (Gamma1 ++ Gamma2) (ESeq e1 e2) B.
-Proof.
-  unfold typed. iIntros (HcopyA He1 He2 vs) "Hctx". simpl.
-  iDestruct (ctx_typed_app with "Hctx") as "[Hctx1 Hctx2]".
-  iApply Seq_wp.
-  iApply (He1 with "Hctx1"); iIntros (v1) "HA".
-  iDestruct (HcopyA with "HA") as "_".
-  iApply (He2 with "Hctx2").
-Qed.
-
-
-
