programs.v
@@ -20,7 +20,7 @@ Definition dec_list : val :=
         let: "x" := fst !"p" in
         let: "l" := snd !"p" in
         if: "x" =: 0
-          then throw tt ()
+          then throw IllegalArgumentException ()
           else "p" <- ("x" -: 1, "l");;
                "dec_list" "l"
     end.
@@ -28,8 +28,9 @@ Definition dec_list : val :=
 Definition main (l : list nat) : val :=
   closure: "_" =>
     let: "l" := alloc_list l () in
-    (dec_list "l";; "l")
-      catch: tt TUnit "_" => "l".
+    dec_list "l"
+      catch: IllegalArgumentException "_" => ();;
+    "l".
 
 Fixpoint is_list (l : list nat) (v : val) : sepProp :=
   match l with
@@ -64,7 +65,7 @@ Lemma dec_list_spec l v :
   {{ vret, @[ vret = () ] **
            @[ Forall positive l ] **
            is_list (map pred l) v }}
-  {{ t vex, @[ t = tt ] ** @[ vex = () ] **
+  {{ t vex, @[ t = IllegalArgumentException ] ** @[ vex = () ] **
             Ex l1 l2, @[ l = l1 ++ 0 :: l2 ] **
                       @[ Forall positive l1 ] **
                       is_list (map pred l1 ++ 0 :: l2) v }}.
@@ -104,11 +105,11 @@ Lemma main_spec l :
 Proof.
   iIntros "_". iApply App_wp. iApply Let_wp.
   iApply (alloc_list_spec with "[//]"); iSplit.
-  - iIntros (v) "Hv". iApply Catch_Lam_wp. iApply Seq_wp.
+  - iIntros (v) "Hv". iApply Seq_wp. iApply Catch_Lam_wp.
     iApply (dec_list_spec with "Hv"); iSplit.
     + iIntros (?) "(% & %Hl & Hv)". iApply Val_wp. eauto with iFrame.
     + iIntros (t ?) "(-> & % & %l1 & %l2 & -> & %Hl1 & Hv)".
-      rewrite tag_dec_eq. iApply Val_wp. eauto with iFrame.
+      rewrite tag_dec_eq. do 2 (iApply Val_wp). eauto with iFrame.
   - by iIntros (??) "?".
 Qed.
 
